src/opt/MemInv.v
@@ -21,100 +21,167 @@ Set Implicit Arguments.
 Module MemInv.
   Definition t := Memory.t.
 
-  Inductive sem (inv:t): forall (local_src local_tgt:Memory.t), Prop :=
+  Inductive sem (inv:t): forall (promise_src promise_tgt:Memory.t), Prop :=
   | sem_intro
-      local_tgt
-      (DISJOINT: Memory.disjoint local_tgt inv):
-      sem inv (Memory.join local_tgt inv) local_tgt
+      promise_tgt
+      (DISJOINT: Memory.disjoint promise_tgt inv):
+      sem inv (Memory.join promise_tgt inv) promise_tgt
   .
 
-  Lemma add
+  Lemma promise
         inv
-        local1_src global1_src
-        local1_tgt global1_tgt local2_tgt global2_tgt
-        (LE1_SRC: Memory.le local1_src global1_src)
-        (LE1_TGT: Memory.le local1_tgt global1_tgt)
+        loc from to msg
+        promise1_src global1_src
+        promise1_tgt global1_tgt promise2_tgt global2_tgt
+        (LE1_SRC: Memory.le promise1_src global1_src)
+        (LE1_TGT: Memory.le promise1_tgt global1_tgt)
         (SIM1: sim_memory global1_src global1_tgt)
-        (INV1: sem inv local1_src local1_tgt)
-        (ADD_TGT: Memory.add local1_tgt global1_tgt local2_tgt global2_tgt):
-    exists local2_src global2_src,
-      <<LE1_SRC: Memory.le local2_src global2_src>> /\
+        (INV1: sem inv promise1_src promise1_tgt)
+        (PROMISE_TGT: Memory.promise promise1_tgt global1_tgt loc from to msg promise2_tgt global2_tgt):
+    exists promise2_src global2_src,
+      <<LE1_SRC: Memory.le promise2_src global2_src>> /\
       <<SIM2: sim_memory global2_src global2_tgt>> /\
-      <<INV2: sem inv local2_src local2_tgt>> /\
-      <<ADD_SRC: Memory.add local1_src global1_src local2_src global2_src>>.
+      <<INV2: sem inv promise2_src promise2_tgt>> /\
+      <<PROMISE_SRC: Memory.promise promise1_src global1_src loc from to msg promise2_src global2_src>>.
   Proof.
-    inv SIM1. inv INV1. inv ADD_TGT. memtac.
-    rewrite <- Memory.join_assoc in SPLITS.
-    apply Memory.splits_join_inv in SPLITS; memtac.
-    exploit Memory.join2_splits; try apply JOINC; memtac.
-    { splits; memtac. }
-    { eapply Memory.splits_disjoint; [|eauto].
-      symmetry. eapply Memory.splits_disjoint; [|eauto].
-      memtac.
-    }
-    i. des. subst. clear JOINC SPLITSA.
-    exists (Memory.join local2_tgt inv).
-    exists (Memory.join (Memory.join (Memory.join local2_tgt inv) addendum) ohs0).
-    splits.
-    - rewrite <- Memory.join_assoc.
-      econs; memtac. repeat (splits; memtac).
-      eapply Memory.splits_disjoint in SPLITSB; memtac.
-    - econs.
-      rewrite <- ? Memory.join_assoc.
-      apply Memory.splits_join; (repeat (splits; memtac)).
-      rewrite (Memory.join_comm _ ohs0).
-      rewrite Memory.join_assoc.
-      apply Memory.splits_join; (repeat (splits; memtac)).
-    - econs. memtac.
-    - rewrite <- (Memory.join_assoc _ addendum ohs0).
-      rewrite (Memory.join_comm addendum ohs0).
-      rewrite (Memory.join_assoc _ ohs0 addendum).
-      econs; (repeat (splits; memtac)).
-      + apply Memory.splits_join; (repeat (splits; memtac)).
-      + eapply Memory.splits_disjoint in SPLITSB; memtac.
-      + eapply Memory.splits_disjoint in SPLITSB; memtac.
+    inv SIM1. inv INV1. inv PROMISE_TGT; memtac.
+    - rewrite <- Memory.join_assoc in SPLITS.
+      apply Memory.splits_join_inv2 in SPLITS; repeat (splits; memtac).
+      exists (Memory.join (Memory.join promise1_tgt inv) (Memory.singleton loc msg LT)).
+      exists (Memory.join (Memory.join (Memory.join promise1_tgt inv) (Memory.singleton loc msg LT)) ohs).
+      splits.
+      + apply Memory.le_join_l. repeat (splits; memtac).
+        symmetry in DISJOINT3. eapply Memory.splits_disjoint in DISJOINT3; [|eauto].
+        memtac.
+      + econs. rewrite <- ? Memory.join_assoc.
+        apply Memory.splits_join; (repeat (splits; memtac)).
+        rewrite (Memory.join_comm _ ohs), Memory.join_assoc.
+        apply Memory.splits_join; (repeat (splits; memtac)).
+      + rewrite <- ? Memory.join_assoc, (Memory.join_comm inv _).
+        rewrite Memory.join_assoc. econs. repeat (splits; memtac).
+        symmetry in DISJOINT3. eapply Memory.splits_disjoint in DISJOINT3; [|eauto].
+        memtac.
+      + econs 1; eauto.
+        * symmetry in DISJOINT3. eapply Memory.splits_disjoint in DISJOINT3; [|eauto].
+          repeat (splits; memtac).
+        * rewrite <- (Memory.join_assoc _ (Memory.singleton _ _ _) ohs).
+          rewrite (Memory.join_comm (Memory.singleton _ _ _) ohs).
+          rewrite Memory.join_assoc.
+          auto.
+    - rewrite Memory.join_assoc, (Memory.join_comm _ promise1_ctx) in SPLITS.
+      rewrite <- ? Memory.join_assoc in SPLITS.
+      apply Memory.splits_join_inv2 in SPLITS; repeat (splits; memtac).
+      rewrite (Memory.join_comm global1_ctx _) in SPLITS.
+      apply Memory.splits_join_inv2 in SPLITS; repeat (splits; memtac).
+      rewrite ? Memory.join_assoc, (Memory.join_comm _ promise1_ctx) in JOIN.
+      rewrite <- ? Memory.join_assoc in JOIN. repeat (splits; memtac).
+      rewrite (Memory.join_comm global1_ctx _) in JOIN. memtac.
+      generalize (Memory.splits_intro loc msg msg0 LT1 LT2). i. des.
+      exists (Memory.join (Memory.join inv promise1_ctx)
+                     (Memory.join (Memory.singleton loc msg LT1) (Memory.singleton loc msg0 LT2))).
+      exists (Memory.join (Memory.join (Memory.join inv ohs0) promise1_ctx)
+                     (Memory.join (Memory.singleton loc msg LT1) (Memory.singleton loc msg0 LT2))).
+      splits.
+      + symmetry in DISJOINT5. symmetry in PROMISE2. symmetry in DISJOINT3.
+        exploit Memory.splits_disjoint; try apply SPLIT; try apply DISJOINT5; eauto. i. memtac.
+        exploit Memory.splits_disjoint; try apply SPLIT; try apply PROMISE2; eauto. i. memtac.
+        exploit Memory.splits_disjoint; try apply SPLIT; try apply DISJOINT3; eauto. i. memtac.
+        repeat apply Memory.le_join;
+          try reflexivity;
+          repeat (splits; memtac).
+        apply Memory.le_join_l. memtac.
+      + econs. rewrite <- Memory.join_assoc.
+        apply Memory.splits_join; (repeat (splits; memtac)).
+      + rewrite <- ? Memory.join_assoc, (Memory.join_comm inv _).
+        econs. repeat (splits; memtac).
+      + econs 2.
+        * rewrite Memory.join_comm, ? Memory.join_assoc. auto.
+        * repeat (splits; memtac).
+        * instantiate (1 := ohs0).
+          rewrite ? Memory.join_assoc, (Memory.join_comm ohs0 _).
+          rewrite <- ? Memory.join_assoc. f_equal.
+          rewrite (Memory.join_comm ohs0 _).
+          rewrite ? Memory.join_assoc. auto.
+        * repeat (splits; memtac).
+        * auto.
+        * rewrite ? Memory.join_assoc, (Memory.join_comm ohs0 _). auto.
   Qed.
 
-  Lemma remove_tgt
-        inv local1_src local1_tgt local2_tgt
+  Lemma confirm_tgt
+        inv promise1_src promise1_tgt promise2_tgt
         loc from to msg
-        (INV: sem inv local1_src local1_tgt)
-        (REMOVE: Memory.remove loc from to msg local1_tgt local2_tgt):
+        (INV: sem inv promise1_src promise1_tgt)
+        (CONFIRM: Memory.confirm promise1_tgt loc from to msg promise2_tgt):
     exists (LT: Time.lt from to),
       <<DISJOINT: Memory.disjoint inv (Memory.singleton loc msg LT)>> /\
-      <<INV: sem (Memory.join inv (Memory.singleton loc msg LT)) local1_src local2_tgt>>.
+      <<INV: sem (Memory.join inv (Memory.singleton loc msg LT)) promise1_src promise2_tgt>>.
   Proof.
-    inv INV. memtac.
+    inv INV. inv CONFIRM. memtac.
     exists LT. splits; memtac.
     rewrite <- Memory.join_assoc, Memory.join_comm.
     econs. memtac. splits; memtac.
   Qed.
 
-  Lemma remove_src
-        inv1 inv2 local1_src local1_tgt
+  Lemma confirm_src
+        inv1 inv2 promise1_src promise1_tgt
         loc from to msg
-        (INV: sem inv1 local1_src local1_tgt)
-        (REMOVE: Memory.remove loc from to msg inv1 inv2):
-    exists (LT: Time.lt from to) local2_src,
-      <<REMOVE: Memory.remove loc from to msg local1_src local2_src>> /\
-      <<INV: sem inv2 local2_src local1_tgt>>.
+        (INV: sem inv1 promise1_src promise1_tgt)
+        (CONFIRM: Memory.confirm inv1 loc from to msg inv2):
+    exists (LT: Time.lt from to) promise2_src,
+      <<CONFIRM: Memory.confirm promise1_src loc from to msg promise2_src>> /\
+      <<INV: sem inv2 promise2_src promise1_tgt>>.
   Proof.
-    inv INV. memtac.
+    inv INV. inv CONFIRM. memtac.
     exists LT. eexists. splits; memtac.
     rewrite Memory.join_assoc. econs; memtac. splits; memtac.
   Qed.
 
-  Lemma sem_bot local:
-    sem Memory.bot local local.
+  Lemma write
+        inv
+        loc from to msg ord
+        promise1_src global1_src
+        promise1_tgt global1_tgt promise2_tgt global2_tgt
+        (LE1_SRC: Memory.le promise1_src global1_src)
+        (LE1_TGT: Memory.le promise1_tgt global1_tgt)
+        (SIM1: sim_memory global1_src global1_tgt)
+        (INV1: sem inv promise1_src promise1_tgt)
+        (RELEASE: Ordering.le Ordering.release ord -> promise1_tgt loc = Cell.bot -> promise1_src loc = Cell.bot)
+        (WRITE_TGT: Memory.write promise1_tgt global1_tgt loc from to msg ord promise2_tgt global2_tgt):
+    exists promise2_src global2_src,
+      <<LE1_SRC: Memory.le promise2_src global2_src>> /\
+      <<SIM2: sim_memory global2_src global2_tgt>> /\
+      <<INV2: sem inv promise2_src promise2_tgt>> /\
+      <<WRITE_SRC: Memory.write promise1_src global1_src loc from to msg ord promise2_src global2_src>>.
   Proof.
-    rewrite <- (Memory.bot_join local) at 1.
+    inv WRITE_TGT.
+    - exploit confirm_tgt; eauto. i. des.
+      exploit confirm_src; eauto.
+      { econs; memtac. }
+      i. des.
+      eexists _, _. splits; try apply INV0; eauto.
+      + eapply Memory.confirm_future; eauto.
+      + econs 1; eauto.
+    - exploit promise; try apply PROMISE; try apply LE1_SRC; eauto. i. des.
+      exploit confirm_tgt; eauto. i. des.
+      exploit confirm_src; eauto.
+      { econs; memtac. }
+      i. des.
+      eexists _, _. splits; try apply INV0; eauto.
+      + eapply Memory.confirm_future; eauto.
+      + econs 2; eauto.
+  Qed.
+
+  Lemma sem_bot promise:
+    sem Memory.bot promise promise.
+  Proof.
+    rewrite <- (Memory.bot_join promise) at 1.
     econs. memtac.
   Qed.
 
   Lemma sem_bot_inv
-        local_src local_tgt
-        (SEM: sem Memory.bot local_src local_tgt):
-    local_src = local_tgt.
+        promise_src promise_tgt
+        (SEM: sem Memory.bot promise_src promise_tgt):
+    promise_src = promise_tgt.
   Proof.
     inv SEM. apply Memory.bot_join.
   Qed.
